theories/binary_format_printer.v
@@ -7,6 +7,8 @@ Require leb128.
 From Stdlib Require Import PeanoNat.
 From mathcomp Require Import ssreflect ssrfun ssrnat ssrbool eqtype seq.
 
+(* TODO: update to actual binary *)
+(* 
 Definition binary_of_number_type (t : number_type) : byte :=
   match t with
   | T_i32 => x7f
@@ -565,3 +567,4 @@ Definition binary_of_module (m : module) : list byte :=
   only_if_non_nil binary_of_elemsec m.(mod_elem) ++
   only_if_non_nil binary_of_codesec m.(mod_funcs) ++
   only_if_non_nil binary_of_datasec m.(mod_data).
+*)
